ESProperties.thy
@@ -1,0 +1,31 @@
+theory ESProperties
+imports EventStructures String
+begin
+  
+lemma aej_subset: "C \<lesssim>\<^sup>*\<^bsub>es\<^esub> D \<Longrightarrow> C \<subseteq> D"
+  apply(simp only: justifies_config_star_inf_def)
+  apply(rule rtrancl_induct[where a=C, where b=D, where r="justifies_config_subset es", 
+        where P="\<lambda>x . C \<subseteq> x"])
+    apply(auto simp add: justifies_config_subset_def)
+  done
+    
+lemma ref_impl: "C \<lesssim>\<^bsub>es\<^esub> C' \<Longrightarrow> C' \<lesssim>\<^bsub>es\<^esub> C'"
+  apply(simp add: justifies_config_inf_def justifies_config_subset_def justifies_config_def)
+  apply clarsimp
+  apply blast
+  done
+      
+lemma add_write_okay: "C' \<lesssim>\<^bsub>es\<^esub> C' \<Longrightarrow> \<not>(is_read ev es) \<Longrightarrow> C' \<lesssim>\<^bsub>es\<^esub> C' \<union> {ev}"
+  apply(simp only: justifies_config_inf_def justifies_config_def)
+  apply(simp (no_asm) add: justifies_config_subset_def justifies_config_def)
+  apply auto
+  apply(simp add: justifies_config_subset_def justifies_config_def)
+  done 
+    
+lemma add_write_really_okay: "C \<lesssim>\<^bsub>es\<^esub> C' \<Longrightarrow> \<not>(is_read ev es) \<Longrightarrow> C' \<lesssim>\<^bsub>es\<^esub> C' \<union> {ev}"
+  apply(rule add_write_okay)
+  apply(rule ref_impl)
+   apply assumption+
+  done
+    
+end
