ExampleEventStructures.thy
@@ -2,22 +2,28 @@ theory ExampleEventStructures
 imports Enum EventStructures Relation Transitive_Closure String
 begin
 
-theorem emptyESValidES: "isValidES empty_ES"
-  apply(auto simp add: isValidES_def empty_ES_def isValidPO_def minimal_def isConfValid_def)
-     apply(rule refl_Id)
-    apply(rule trans_Id)
-   apply(rule antisym_Id)
-   apply(simp_all add: symmetriccl_def symmetric_symmetriccl)
-   apply(simp_all add: symmetric_def trans_def irrefl_def)
-  apply(auto)
+theorem emptyESValidES: "isValidES \<I>"
+  apply(auto simp add: isValidES_def initialES_def isValidPO_def minimal_def isConfValid_def)
+  apply(rule refl_Id)
+     apply(rule trans_Id)
+    apply(rule antisym_Id)
+   apply(simp add: symmetriccl_def symmetric_symmetriccl)
+   apply(simp add: sym_def trans_def irrefl_def)
+  apply(simp add: trans_rtrancl)
   done
-
-theorem emptyESWellJustified: "well_justified empty_ES {}"
+    
+lemma initialConfig_no_read: "\<not> is_read x \<I>"
+  apply(simp add: initialES_def)
+  apply(simp add: is_read_def)
+  done
+    
+theorem emptyESWellJustified: "well_justified \<I> \<C>"
   apply(auto simp add: well_justified_def)
   apply(rule emptyESValidES)
-  apply(auto simp add: empty_ES_def justified_def ae_justifies_subset_star_def)
+   apply(auto simp add: justified_def ae_justifies_subset_star_def)
   done
-
+    
+    
 theorem emptyESJustEmptyES: "{} \<lesssim>\<^bsub>es\<^esub> {}"
   apply(auto simp add: justifies_config_inf_def justifies_config_subset_def justifies_config_def)
   done
