RelationalLemmas.thy
@@ -1,0 +1,27 @@
+theory RelationalLemmas
+  imports Main Relation Transitive_Closure
+begin
+  
+definition symmetric:: "'a rel \<Rightarrow> bool" where
+  "symmetric r \<equiv> \<forall>a b . (a, b) \<in> r \<longleftrightarrow> (b, a) \<in> r"
+      
+definition symmetriccl:: "'a rel \<Rightarrow> 'a rel" where
+  "symmetriccl r \<equiv> {(y, x) . (x, y) \<in> r} \<union> r"
+  
+lemma symmetric_symmetriccl: "\<forall>r . sym (symmetriccl r)"
+  apply(simp add: sym_def symmetriccl_def)
+  done
+    
+lemma symm_imp_symm_trancl: "sym r \<longrightarrow> sym (r\<^sup>+)"
+  apply(auto simp add: sym_def)
+  apply(erule trancl.induct[where ?P = "\<lambda>a b. (b, a) \<in> r\<^sup>+"])
+  apply auto
+   apply(meson trancl_into_trancl2)
+  done
+
+lemma symm_pc: "sym ((symmetriccl r)\<^sup>+)"
+  apply(simp add: sym_def)
+  by (meson  symm_imp_symm_trancl sym_def symmetric_symmetriccl)
+
+end
+  
